Cast level LE as basic

Gt3/HasTy/Basic.lean
@@ -72,9 +72,9 @@ inductive Ctx.HasTy : Ctx → Tm 0 → Tm 0 → Prop
     (hA : HasTy Γ (.univ ℓ) A)
     (ha : HasTy Γ A a)
     : HasTy Γ .unit (.has_ty A a)
-  | cast_level {Γ} {ℓ A}
-    (hA : HasTy Γ (.univ ℓ) A)
-    : HasTy Γ (.univ (ℓ + 1)) A
+  | cast_level_le {Γ} {lo hi A} (h : lo ≤ hi)
+    (hA : HasTy Γ (.univ lo) A)
+    : HasTy Γ (.univ hi) A
   | cast {Γ} {A A' a : Tm 0}
     (hA : TyEq Γ A A') (ha : HasTy Γ A a)
     : HasTy Γ A' a
@@ -85,11 +85,8 @@ inductive Ctx.HasTy : Ctx → Tm 0 → Tm 0 → Prop
 theorem Ctx.HasTy.cast' {Γ ℓ A A' a} (hA : JEq Γ (.univ ℓ) A A') (ha : HasTy Γ A a)
   : HasTy Γ A' a := .cast hA.ty_eq ha
 
-theorem Ctx.HasTy.cast_level_le {Γ A lo hi} (h : lo ≤ hi) (hA : HasTy Γ (.univ lo) A)
-  : HasTy Γ (.univ hi) A := by
-  induction h with
-  | refl => exact hA
-  | step hlt ih => exact .cast_level ih
+theorem Ctx.HasTy.cast_level {Γ A ℓ} (hA : HasTy Γ (.univ ℓ) A) : HasTy Γ (.univ (ℓ + 1)) A
+  := .cast_level_le (by simp) hA
 
 theorem Ctx.HasTy.ok {Γ A a} (h : HasTy Γ A a) : Ok Γ := by induction h <;> assumption
 
@@ -97,7 +94,7 @@ theorem Ctx.HasTy.not {Γ φ} (hφ : HasTy Γ (.univ 0) φ) : HasTy Γ (.univ 0)
   := .eqn hφ (.empty hφ.ok)
 
 theorem Ctx.HasTy.refl {Γ A a} (h : HasTy Γ A a) : JEq Γ A a a := by induction h with
-  | cast_level _ IA => exact IA.cast_level
+  | cast_level_le hℓ _ IA => exact IA.cast_level_le hℓ
   | cast hA _ Ia => exact Ia.cast hA
   | transfer _ hB IA => exact IA.transfer' hB
   | _ => jeq_congr_f <;> assumption
